chore: think of how to reduce sext/zext to existing ops

SSA/Experimental/Bits/Fast/ZextSext.lean
@@ -6,28 +6,28 @@ inductive NatExpr (n : Nat) : Type
 | var : (v : Fin n) → NatExpr n
 | add : NatExpr n → NatExpr n → NatExpr n
 
-def NatExpr.eval (e : NatExpr n) (env : Fin n → Nat) : Nat :=
+def NatExpr.toDefEqBV (e : NatExpr n) (env : Fin n → Nat) : Nat :=
   match e with
   | .var v => env v
-  | .add e1 e2 => NatExpr.eval e1 env + NatExpr.eval e2 env
+  | .add e1 e2 => NatExpr.toDefEqBV e1 env + NatExpr.toDefEqBV e2 env
 
 -- inductive NatPredicate (n : Nat) : Type
 -- | eq : NatExpr n → NatExpr n → NatPredicate n
 
--- def NatPredicate.eval (env : Fin n → Nat) : NatPredicate n → Prop
---   | .eq e1 e2 => NatExpr.eval e1 env = NatExpr.eval e2 env
+-- def NatPredicate.toDefEqBV (env : Fin n → Nat) : NatPredicate n → Prop
+--   | .eq e1 e2 => NatExpr.toDefEqBV e1 env = NatExpr.toDefEqBV e2 env
 --
 -- def NatPredicate.decide : NatPredicate n → Bool := sorry
 --
--- theorem NatPredicate.decide_iff_eval (p : NatPredicate n) :
---   (∀ (env : Fin n → Nat), p.eval env) ↔
+-- theorem NatPredicate.decide_iff_toDefEqBV (p : NatPredicate n) :
+--   (∀ (env : Fin n → Nat), p.toDefEqBV env) ↔
 --   (p.decide = true) := sorry
 
 -- theorem foo : ∀ (n m : Nat), n + m = m + n := by
 --   -- (NatPredicate.eq (NatExpr.add (NatExpr.var 0) (NatExpr.var 1))
---   --   (NatExpr.add (NatExpr.var 1) (NatExpr.var 0))).eval (...)
+--   --   (NatExpr.add (NatExpr.var 1) (NatExpr.var 0))).toDefEqBV (...)
 --   -- revert env
---   -- apply NatPredicate.decide_iff_eval |>.mpr (by rfl)
+--   -- apply NatPredicate.decide_iff_toDefEqBV |>.mpr (by rfl)
 --   sorry
 
 namespace BV
@@ -41,29 +41,35 @@ inductive BVExpr (ctx : BVTyCtx natCard bvCard) : (NatExpr natCard) → Type
 | append (a : BVExpr ctx v) (b : BVExpr ctx w) : BVExpr ctx (.add v w)
 
 abbrev BVEnv (tyCtx : BVTyCtx natCard bvCard) (natEnv : Fin natCard → Nat) :=
-  (v : Fin bvCard) → BitVec ((tyCtx v).eval natEnv)
+  (v : Fin bvCard) → BitVec ((tyCtx v).toDefEqBV natEnv)
 
-def BVExpr.eval {natEnv : Fin n → Nat} (bvEnv : BVEnv bvCard natEnv) :
-  BVExpr bvCard w → BitVec (w.eval natEnv)
+def BVExpr.toDefEqBV {natEnv : Fin n → Nat} (bvEnv : BVEnv bvCard natEnv) :
+  BVExpr bvCard w → BitVec (w.toDefEqBV natEnv)
 | .var v => bvEnv v
-| .add a b => a.eval bvEnv + b.eval bvEnv
-| .append a b => a.eval bvEnv ++ b.eval bvEnv
+| .add a b => a.toDefEqBV bvEnv + b.toDefEqBV bvEnv
+| .append a b => a.toDefEqBV bvEnv ++ b.toDefEqBV bvEnv
 
 inductive BVPredicate (ctx : BVTyCtx natCard bvCard) : Type
 | eq (a : BVExpr ctx w) (b : BVExpr ctx w)
 
-def BVPredicate.eval {natEnv : Fin natCard → Nat} {ctx : BVTyCtx natCard bvCard}
+def BVPredicate.toDefEqBV {natEnv : Fin natCard → Nat} {ctx : BVTyCtx natCard bvCard}
     (bvEnv : BVEnv ctx natEnv) :
   BVPredicate ctx → Prop
-| .eq a b => a.eval bvEnv = b.eval bvEnv
+| .eq a b => a.toDefEqBV bvEnv = b.toDefEqBV bvEnv
 
 def BVPredicate.decide (ctx : BVTyCtx natCard bvCard) :
   BVPredicate ctx → Bool 
 | .eq a b => false
 
-theorem BVPredicate.eval_of_decide (ctx : BVTyCtx natCard bvCard)
+
+/-- Rewrite rule to express msb in terms of slt. -/
+theorem BitVec.msb_iff_slt_zero (bv : BitVec w) :
+  bv.msb = true ↔ bv.slt 0#w = true := by
+  simp [BitVec.msb_eq_toInt, BitVec.slt_eq_decide]
+
+theorem BVPredicate.toDefEqBV_of_decide (ctx : BVTyCtx natCard bvCard)
     (p : BVPredicate ctx) (h : p.decide = true) :
-  ∀ (bvEnv : BVEnv ctx natEnv), p.eval bvEnv := by
+  ∀ (bvEnv : BVEnv ctx natEnv), p.toDefEqBV bvEnv := by
   sorry
 
 inductive Expr
